### Ejercicio 7

$f_1(x,y) = (\exists t)(\text{STEP}^{(1)}(x,t,y) = 1)$

$f_2(x) = (\exists \langle t, y \rangle)(\text{STEP}^{(1)}(x,t,y) = 1)$

$f_3(x,y) = (\exists \langle t, z \rangle)
(\text{STEP}^{(1)}(x,t,z) = 1 \land r(\text{SNAP}^{(1)}(x,t,z))[0] = y)$

$f_4(x,y) = (\exists \langle t_1, \langle t_2, z \rangle \rangle)(\text{STEP}^{(1)}(x,t_1,z) + \text{STEP}^{(1)}(y,t_2,z) = 2)$

$f_5(x) = (\exists \langle t, z \rangle)
(\text{STEP}^{(1)}(x,t,z) = 1 \land r(\text{SNAP}^{(1)}(x,t,z))[0] = z)$

$f_6(x,y) = (\exists \langle t_1, \langle t_2, z \rangle \rangle)
(r(\text{SNAP}^{(1)}(x,t_1,z))[0] = r(\text{SNAP}^{(1)}(y,t_2,z))[0])$

$f_7(x,y) = (\exists \langle t,z \rangle)
(\text{STEP}^{(1)}(x,t,y) \neq 0 \land r(\text{SNAP}^{(1)}(y,t_2,z))[0] = w \land esPrimo(w))$

$f_8(x,y) = (\exists \langle t, \langle T, z \rangle \rangle)
(\text{STEP}^{(1)}(x,t,y) \neq 0 \land r(\text{SNAP}^{(1)}(y,t_2,z))[0] \neq 0 )$